---
title: Linear codes
date: 2024-02-28
---


\newcommand{\F}{\mathbb{F}}
\newcommand{\Z}{\mathbb{Z}}
\newcommand{\NN}{\mathbb{N}}
\newcommand{\CC}{\mathbb{C}}
\newcommand{\e}{\mathbf{e}}
\newcommand{\h}{\mathbf{h}}
\newcommand{\bb}{\mathbf{b}}
\newcommand{\vv}{\mathbf{v}}
\newcommand{\xx}{\mathbf{x}}

\newcommand{\uu}{\mathbf{u}}
\newcommand{\ww}{\mathbf{w}}

\newcommand{\Null}{\operatorname{Null}}
\newcommand{\Hom}{\operatorname{Hom}}

\newcommand{\weight}{\operatorname{weight}}

\newcommand{\PP}{\mathbb{P}}

\newcommand{\dist}{\operatorname{dist}}
\newcommand{\floor}[1]{\lfloor #1 \rfloor}

\newcommand{\tr}{\operatorname{tr}}

# Dual codes and weight enumerators

Consider a $[n,k]_q$-code $C$, and write $$\langle \cdot, \cdot
\rangle: \F_q^n \times \F_q^n \to \F_q$$ for the *standard inner
product*; if $\e_1,\cdots,\e_n$ are the standard basis vectors, then
we have $$\langle \e_i,\e_j \rangle = \delta_{ij}.$$

We write $C^\perp$ for the *dual code* to $C$ defined by the rule
$$C^\perp = \{ \ww \in \F_q^n \mid \langle \ww, C \rangle = 0\} =
\{ \ww \in \F_q^n \mid \langle \ww,x \rangle = 0 \quad \forall x \in C\}.$$

Observe that the natural mapping
$$\F_q^n \to C^*$$
given by $\ww \mapsto \langle \cdot,\ww \rangle = (x \mapsto \langle x, \ww \rangle)$
is a surjection with kernel $C^\perp$. It thus follows that
$$\dim C^\perp = n - \dim C^* = n - \dim C = n -k.$$

In particular, $C^\perp$ is an $[n,n-k]_q$-code.

**Remark**
:   If $C = C^\perp$, we say that $C$ is *self-dual*. Note that if $C$
    is self dual we must have $k = n-k$ so that $n = 2k$ is *even*.
	
	For example, the following is a self-dual $[8,4]_2$ code.
	
	``` python
	k = GF(2)
    V = VectorSpace(k,8)
    
    C = V.subspace([V([1,0,0,0,1,1,1,0]),
                    V([0,1,0,0,1,1,0,1]),
                    V([0,0,1,0,1,0,1,1]),
                    V([0,0,0,1,0,1,1,1])])
    
	# generator matrix
    G = MatrixSpace(k,4,8).matrix(C.basis())
	
	G * G.T
	=>
	
	[0 0 0 0]
    [0 0 0 0]
    [0 0 0 0]
    [0 0 0 0]
    ```

    We see for this example that $C \subset C^\perp$ and thus $C =
	C^\perp$ since $\dim C = 4 = 8-4 = \dim C^\perp$.


## Weight enumerators

Consider the polynomial with natural-number coefficients
$$A(T) = \sum_{\uu \in C} T^{\weight(\uu)} \in \NN[T].$$

We evidently have 
$$A(T) = \sum_{i=0}^n A_i T^i = 1 + \sum_{i=1}^n A_i T^i$$
where $A_i = \#\{\uu \in C \mid \weight(\uu) = i\}$ (note that $A_0 = 1$).
We call $A(T)$ the *weight-enumerator* polynomial of $C$.

**Example**
:  Consider the self-dual $[8,4]_2$-code $C$ introduced above;
   namely:
   
   ``` python
	k = GF(2)
    V = VectorSpace(k,8)
    
    C = V.subspace([V([1,0,0,0,1,1,1,0]),
                    V([0,1,0,0,1,1,0,1]),
                    V([0,0,1,0,1,0,1,1]),
                    V([0,0,0,1,0,1,1,1])])
   ```
   
   We  compute its weight-enumerator:
   
   ``` python
   R.<T> = PolynomialRing(ZZ)
    
   ## compute the weight enumerator, as an element of R
   def WE(C):
       return sum([ T^weight(c) for c in C ])
   
   WE(C)
   =>
   T^8 + 14*T^4 + 1	
   ```

Write $A^\perp(T)$ for the weight enumerator. We are going to prove a formula
relating $A(T)$ and $A^\perp(T)$ due to McWilliams.

The proof involves some *character theory*. We need a few extra tools.

## Characters of $\F_q$-vector spaces.

Let $\tr:\F_q \to \F_p$ be the *trace map*.

For any finite degree field extension $E \supset F$ we have a trace mapping
$\tr:E \to F$; for $\alpha \in E$,
$\tr(\alpha)$ is the trace of the $F$-linear mapping $E \to E$ given by
$x \mapsto \alpha x$.

**Proposition**
:   If $E \supset F$ is a finite Galois extension, and if $\Gamma =
    \operatorname{Gal}(E/F)$ is the *galois group*, then
	for $\alpha \in E$ we have
	$$\tr(\alpha) = \sum_{\sigma \in \Gamma} \sigma(\alpha).$$


**Proposition**
:   If $q = p^2$, then $\tr:\F_q \to \F_p$ is given by the formula
    $$\tr(\alpha) = \alpha + \alpha^p + \alpha^{p^2} + \cdots  + \alpha^{p^{s-1}}.$$


The importance to us of the trace mapping is this: we know how to
describe complex characters of $\F_p$, and we use these together with
the trace to describe complex characters of $\F_q$.

Fix $\zeta_p = \exp\left ( \dfrac{2\pi i}{p} \right) \in \CC^\times.$

For a vector $\uu \in \F_q^n$, we define a group homomorphism
("character") $$\chi_\uu:\F_q^n \to \CC^\times$$ by the rule
$$\chi_\uu(\vv) = \zeta_p^{\tr(\langle \uu, \vv \rangle)} = \exp\left
( \dfrac{2\pi i}{p} \tr( \langle \uu,\vv \rangle)\right)$$

Observe that since $\tr(\alpha) \in \F_p = \Z/p\Z$ for $\alpha \in \F_q$,
the complex number 
$\zeta_p^{\tr(\alpha)}$ is always *well-defined*.

**Remark**
:  Arguing as in an earlier homework exercise, it is easy to see that
   $\widehat{\F_q^n} = \Hom(\F_q^n,\CC^\times) =  \{ \chi_\uu \mid \uu \in \F_q^n \}$.


For a finite abelian group $A$, recall that we write $$\langle \chi,\phi \rangle_A
= \dfrac{1}{|A|} \sum_{a \in A} \chi(a) \overline{\phi(a)}$$ for the
*character inner product*; here $\chi,\phi \in \widehat{A} = \Hom(A,\CC^\times)$.

We have the following result from *character theory*:

**Proposition**
:  For $\xx \in \F_q^n$, we have
   $$\sum_{\uu \in C}   \chi_\uu(\xx)  \left \{
   \begin{matrix}
   0 & \text{if $\xx \not \in C^\perp$} \\  |C| & \text{if $\xx \in C^\perp$}
   \end{matrix}
   \right .$$

**Proof**
:   We know that $\chi_\uu\mid_C$ is a character of $C$; i.e. an element of $\widehat{C}$.

    Now,
	\begin{align*}
	\sum_{\uu \in C} \chi_\uu(\xx) &= \sum_{\uu \in C} \zeta_p^{\tr(\langle \uu, \xx \rangle )} 
	= \sum_{u \in C} \chi_\xx(\uu) \\
	&= |C| \langle \chi_\xx, \mathbf{1}_C \rangle_C \\
	&= \left \{ \begin{matrix} |C|  & \text{if $\chi_\xx = \mathbf{1}_C$} \\ 
	0 & \text{otherwise}
	\end{matrix} \right .
	\end{align*}
    where $\mathbf{1}_C$ denotes the trivial homomorphism $C \to \CC^\times$.

    Now the result follows from the observation that $\chi_\xx = \mathbf{1}_C$ if and only
	$\langle \xx,\uu \rangle = 0 \quad \forall \uu \in C$ if and only if $\xx \in C^\perp$.

**Theorem** *(McWilliams' Identity)*
:   If $C$ is an $[n,k]_q$-code, then
    $$q^k A^\perp(T) = (1 + (q-1)T)^n \cdot A\left(\dfrac{1-T}{1+(q-1)T}\right).$$

**Proof**
:   see [@ballCourseAlgebraicErrorCorrecting2020, Theorem 4.13 page 56]

# Bibliography

::: {.refs}
:::
